Betree/BetreeInv.i.dfy
@@ -195,7 +195,7 @@ module BetreeInv {
     && BI.OpTransaction(k, s, s', QueryOps(LookupQuery(key, value, lookup)))
   }
 
-  predicate SuccQuery(k: BI.Constants, s: BI.Variables, s': BI.Variables, key: Key, res: UI.SuccResult, lookup1: Lookup, lookup2: Lookup)
+  predicate SuccQuery(k: BI.Constants, s: BI.Variables, s': BI.Variables, key: Key, res: seq<UI.SuccResult>, lookup1: Lookup, lookup2: Lookup)
   {
     && ValidSuccQuery(BetreeSpec.SuccQuery(key, res, lookup1, lookup2))
     && BI.Reads(k, s, SuccQueryReads(BetreeSpec.SuccQuery(key, res, lookup1, lookup2)))
